full QED for quarter round

examples/riscv/chacha/chacha_quarter_round_propScript.sml
@@ -1,6 +1,10 @@
 open HolKernel boolLib Parse bossLib;
 
-open markerTheory;
+open markerTheory wordsTheory wordsLib;
+
+open addressTheory;
+
+open holba_auxiliaryTheory;
 
 open bir_programSyntax bir_program_labelsTheory;
 open bir_immTheory bir_valuesTheory bir_expTheory bir_exp_immTheory;
@@ -26,6 +30,8 @@ open program_logicSimps;
 open bir_env_oldTheory;
 open bir_program_varsTheory;
 
+open HolBACoreSimps;
+
 open chachaTheory;
 open chacha_specTheory;
 open chacha_symb_transf_quarter_roundTheory;
@@ -35,15 +41,28 @@ val _ = new_theory "chacha_quarter_round_prop";
 Definition riscv_chacha_line_pre_def:
  riscv_chacha_line_pre (pre_a:word32)
   (pre_b:word32) (pre_d:word32)
-  (m:riscv_state) : bool = T  
+  (m:riscv_state) : bool =
+ (n2w (w2n (m.c_gpr m.procID 10w)) = pre_a /\
+  n2w (w2n (m.c_gpr m.procID 22w)) = pre_b /\
+  n2w (w2n (m.c_gpr m.procID 26w)) = pre_d)
+End
+
+Definition riscv_chacha_line_exp_fst_def:
+ riscv_chacha_line_exp_fst (pre_a:word32) (pre_b:word32) : word32 =
+  pre_a + pre_b
+End
+
+Definition riscv_chacha_line_exp_snd_def:
+ riscv_chacha_line_exp_snd pre_a pre_d (s:word32) : word32 =
+  ((pre_a ?? pre_d) <<~ s) || ((pre_a ?? pre_d) >>>~ (32w - s))
 End
 
 Definition riscv_chacha_line_post_def:
- riscv_chacha_line_post (pre_a:word32)
-  (pre_b:word32) (pre_d:word32)
-  (m:riscv_state) : bool = T  
+ riscv_chacha_line_post (pre_a:word32) (pre_b:word32) (pre_d:word32)
+  (m:riscv_state) : bool =
+ (n2w (w2n (m.c_gpr m.procID 20w)) = riscv_chacha_line_exp_fst pre_a pre_b /\
+  n2w (w2n (m.c_gpr m.procID 10w)) = riscv_chacha_line_exp_snd (riscv_chacha_line_exp_fst pre_a pre_b) pre_d 16w)
 End
-
 
 (* ------------------------------------- *)
 (* Connecting RISC-V and BSPEC contracts *)
@@ -53,8 +72,17 @@ Theorem chacha_line_riscv_pre_imp_bspec_pre_thm:
  bir_pre_riscv_to_bir
   (riscv_chacha_line_pre pre_a pre_b pre_d)
   (bspec_chacha_line_pre pre_a pre_b pre_d)
-Proof
- cheat
+Proof 
+ rw [bir_pre_riscv_to_bir_def,riscv_chacha_line_pre_def,bspec_chacha_line_pre_def] >-
+  (rw [bir_is_bool_exp_REWRS,bir_is_bool_exp_env_REWRS] >>
+   FULL_SIMP_TAC (std_ss++holBACore_ss) [bir_typing_expTheory.type_of_bir_exp_def]) >>
+ FULL_SIMP_TAC (std_ss++holBACore_ss) [
+  riscv_bmr_rel_EVAL,bir_val_TF_bool2b_DEF,
+  bool2b_def,
+  bool2w_def,
+  w2w_n2w_w2n_64_32
+ ] >>
+ EVAL_TAC
 QED
 
 Theorem chacha_line_riscv_post_imp_bspec_post_thm:
@@ -63,7 +91,45 @@ Theorem chacha_line_riscv_post_imp_bspec_post_thm:
    (\l. (bspec_chacha_line_post pre_a pre_b pre_d))
    ls
 Proof
- cheat
+ rw [bir_post_bir_to_riscv_def,riscv_chacha_line_post_def,bspec_chacha_line_post_def] >>
+ Cases_on `bs` >>
+ Cases_on `b0` >>
+ FULL_SIMP_TAC (std_ss++holBACore_ss) [
+  bir_envTheory.bir_env_read_def, bir_envTheory.bir_env_check_type_def,
+  bir_envTheory.bir_env_lookup_type_def, bir_envTheory.bir_env_lookup_def,bir_eval_bin_pred_def
+ ] >> 
+ Q.ABBREV_TAC `g = ?z. f "x20" = SOME z /\ BType_Imm Bit64 = type_of_bir_val z` >>
+ Cases_on `g` >> FULL_SIMP_TAC (std_ss++holBACore_ss) [] >>
+ fs [Abbrev_def] >>
+ fs [] >>
+ Cases_on `z` >> fs [type_of_bir_val_def] >>
+
+ Q.ABBREV_TAC `g = ?z. f "x10" = SOME z /\ type_of_bir_val z = BType_Imm Bit64` >>
+ Cases_on `g` >> FULL_SIMP_TAC (std_ss++holBACore_ss) [] >>
+ fs [Abbrev_def] >>
+ fs [] >>
+ Cases_on `z` >> fs [type_of_bir_val_def] >>
+ 
+ FULL_SIMP_TAC (std_ss++holBACore_ss) [bir_eval_cast_def,bir_cast_def,bool2b_def,bool2w_def,b2n_def] >>
+
+ Cases_on `b'` >> fs [type_of_bir_imm_def] >>
+ 
+ Cases_on `b''` >> fs [type_of_bir_imm_def] >>
+ 
+ fs [bir_val_true_def,b2n_def] >>
+
+ Cases_on `n2w (w2n c) = pre_a + pre_b` >> fs [] >>
+
+ Cases_on `n2w (w2n c') =
+           pre_a ≪ 16 + pre_b ≪ 16 ⊕ pre_d ≪ 16 ‖
+           pre_d ⋙ 16 ⊕ (pre_a + pre_b) ⋙ 16` >> fs [] >>
+
+ rw [riscv_chacha_line_exp_fst_def,riscv_chacha_line_exp_snd_def] >>
+
+ FULL_SIMP_TAC (std_ss++holBACore_ss) [riscv_bmr_rel_EVAL,bir_envTheory.bir_env_read_def,
+  bir_envTheory.bir_env_check_type_def, bir_envTheory.bir_env_lookup_type_def,
+  bir_envTheory.bir_env_lookup_def,bir_eval_bin_pred_def] >>
+ rw []
 QED
 
 (* --------------------- *)
